Nearly finished cleanup of PairingHeap. Partial cleanup of selection sort, leftist heaps and splay heaps.

DS/LeftistHeap2.v
@@ -16,20 +16,20 @@ match t with
     | node n _ _ _ => n
 end.
 
-Inductive elem {A : Type} (x : A) : RSTree A -> Prop :=
-    | elem_root : forall (n : nat) (l r : RSTree A),
-        elem x (node n x l r)
-    | elem_left : forall (n : nat) (v : A) (l r : RSTree A),
-        elem x l -> elem x (node n v l r)
-    | elem_right : forall  (n : nat) (v : A) (l r : RSTree A),
-        elem x r -> elem x (node n v l r).
+Inductive Elem {A : Type} (x : A) : RSTree A -> Prop :=
+    | Elem_root : forall (n : nat) (l r : RSTree A),
+        Elem x (node n x l r)
+    | Elem_left : forall (n : nat) (v : A) (l r : RSTree A),
+        Elem x l -> Elem x (node n v l r)
+    | Elem_right : forall  (n : nat) (v : A) (l r : RSTree A),
+        Elem x r -> Elem x (node n v l r).
 
 Inductive isHeap {A : LinDec} : RSTree A -> Prop :=
     | isHeap_empty : isHeap empty
     | isHeap_node :
         forall  (n : nat) (v : A) (l : RSTree A) (r : RSTree A),
-          (forall x : A, elem x l -> v ≤ x) -> isHeap l ->
-          (forall x : A, elem x r -> v ≤ x) -> isHeap r ->
+          (forall x : A, Elem x l -> v ≤ x) -> isHeap l ->
+          (forall x : A, Elem x r -> v ≤ x) -> isHeap r ->
             isHeap (node n v l r).
 
 Lemma isHeap_inv_l :
@@ -49,22 +49,22 @@ Qed.
 Lemma isHeap_inv_leq :
   forall (A : LinDec) (n : nat) (v : A) (l r : RSTree A),
     isHeap (node n v l r) -> forall x : A,
-      elem x (node n v l r) -> v ≤ x.
+      Elem x (node n v l r) -> v ≤ x.
 Proof.
   do 2 inversion 1; subst; auto.
 Qed.
 
 Hint Resolve isHeap_inv_l isHeap_inv_r : core.
 
-Inductive left_biased {A : LinDec} : RSTree A -> Prop :=
-    | left_biased_empty : left_biased empty
-    | left_biased_node :
+Inductive LeftBiased {A : LinDec} : RSTree A -> Prop :=
+    | LeftBiased_empty : LeftBiased empty
+    | LeftBiased_node :
         forall (v : A) (l r : RSTree A),
           right_spine r <= right_spine l ->
-          left_biased l -> left_biased r ->
-            left_biased (node (S (right_spine r)) v l r).
+          LeftBiased l -> LeftBiased r ->
+            LeftBiased (node (S (right_spine r)) v l r).
 
-Hint Constructors RSTree elem isHeap left_biased : core.
+Hint Constructors RSTree Elem isHeap LeftBiased : core.
 
 Ltac lh x :=
   let t := fresh "t" in
@@ -79,49 +79,18 @@ match t with
     | node _ v _ _ => Some v
 end.
 
-(*Theorem getMin_spec :
-  forall (A : LinDec) (h : LeftistHeap A) (m : A),
-    getMin h = Some m -> forall x : A, elem x h -> m ≤ x.
-Proof.
-  lh h; inversion 1; subst. inversion 1; auto.
-Qed.
-
-Definition emptyHeap {A : LinDec} : LeftistHeap A.
-Proof.
-  split with (tree := empty); auto.
-Defined.
-
-Theorem emptyHeap_spec :
-  forall (A : LinDec) (x : A), ~ elem x emptyHeap.
-Proof.
-  inversion 1.
-Qed.*)
-
 Definition singleton' {A : Type} (x : A)
   : RSTree A := node 1 x empty empty.
-
-(*Definition singleton {A : LinDec} (x : A) : LeftistHeap A.
-Proof.
-  split with (tree := singleton' x);
-  constructor; auto; inversion 1.
-Defined.*)
 
 Ltac elem :=
   intros; unfold singleton' in *; cbn in *; subst; repeat
 match goal with
-    | |- elem ?x (node ?x _ _) => constructor
-    | H : elem _ empty |- _ => inv H
-    | H : elem _ (node _ empty empty) |- _ => inv H
-    | H : elem _ _ /\ elem _ _ |- _ => destruct H
-    | H : elem _ _ \/ elem _ _ |- _ => destruct H
+    | |- Elem ?x (node ?x _ _) => constructor
+    | H : Elem _ empty |- _ => inv H
+    | H : Elem _ (node _ empty empty) |- _ => inv H
+    | H : Elem _ _ /\ Elem _ _ |- _ => destruct H
+    | H : Elem _ _ \/ Elem _ _ |- _ => destruct H
 end; auto.
-
-(*Theorem singleton_spec :
-  forall (A : LinDec) (x y : A),
-    elem x (singleton y) <-> x = y.
-Proof.
-  split; elem.
-Qed.*)
 
 Definition balance {A : Type} (v : A) (l r : RSTree A) : RSTree A :=
   if right_spine r <=? right_spine l
@@ -149,7 +118,7 @@ Proof.
   intros. cbn. lia.
 Qed.
 
-Lemma balance_size:
+Lemma size_balance:
   forall (A : Type) (n : nat) (v : A) (l r : RSTree A),
     size (balance v l r) = size (node n v l r).
 Proof.
@@ -158,26 +127,26 @@ Proof.
     cbn. lia.
 Qed.
 
-Lemma balance_elem :
+Lemma Elem_balance :
   forall (A : Type) (n : nat) (x v : A) (l r : RSTree A),
-    elem x (balance v l r) <-> elem x (node n v l r).
+    Elem x (balance v l r) <-> Elem x (node n v l r).
 Proof.
   intros. balance; split; intro; inv H.
 Qed.
 
-Theorem balance_isHeap :
+Theorem isHeap_balance :
   forall (A : LinDec) (n : nat) (v : A) (l r : RSTree A),
-    (forall x : A, elem x l -> v ≤ x) ->
-    (forall x : A, elem x r -> v ≤ x) ->
+    (forall x : A, Elem x l -> v ≤ x) ->
+    (forall x : A, Elem x r -> v ≤ x) ->
       isHeap l -> isHeap r -> isHeap (balance v l r).
 Proof.
   intros; balance; constructor; elem.
 Qed.
 
-Theorem balance_left_biased :
+Theorem LeftBiased_balance :
   forall (A : LinDec) (v : A) (l r : RSTree A),
-    left_biased l -> left_biased r ->
-      left_biased (balance v l r).
+    LeftBiased l -> LeftBiased r ->
+      LeftBiased (balance v l r).
 Proof.
   intros. balance; constructor; cbn in *; dec.
 Qed.
@@ -203,111 +172,84 @@ Defined.
 
 Arguments merge' [x] _.
 
-Lemma elem_merge' :
+Lemma Elem_merge' :
   forall (A : LinDec) (x : A) (t1 t2 : RSTree A),
-    elem x (merge' (t1, t2)) -> elem x t1 \/ elem x t2.
+    Elem x (merge' (t1, t2)) -> Elem x t1 \/ Elem x t2.
 Proof.
   intros. remember (t1, t2) as p. revert x t1 t2 Heqp H.
   functional induction @merge' A p; inv 1; intros.
-    rewrite balance_elem in H. inv H. edestruct IHr; eauto.
-    rewrite balance_elem in H. inv H. edestruct IHr; eauto.
+    rewrite Elem_balance in H. inv H. edestruct IHr; eauto.
+    rewrite Elem_balance in H. inv H. edestruct IHr; eauto.
     Unshelve. all: auto.
 Qed.
 
-Lemma elem_merge'_v2 :
+Lemma Elem_merge'_v2 :
   forall (A : LinDec) (x : A) (t1 t2 : RSTree A),
-    elem x t1 \/ elem x t2 -> elem x (merge' (t1, t2)).
+    Elem x t1 \/ Elem x t2 -> Elem x (merge' (t1, t2)).
 Proof.
   intros. remember (t1, t2) as p. revert x t1 t2 Heqp H.
   functional induction @merge' A p; inv 1;
-  elem; rewrite balance_elem.
-    inv H. apply elem_right.
+  elem; rewrite Elem_balance.
+    inv H. apply Elem_right.
       eapply IHr; try ((left + right); eauto); reflexivity.
-    apply elem_right.
+    apply Elem_right.
       eapply IHr; try ((left + right); eauto); reflexivity.
-    apply elem_right.
+    apply Elem_right.
       eapply IHr; try ((left + right); eauto); reflexivity.
-    inv H. apply elem_right.
+    inv H. apply Elem_right.
       eapply IHr; try ((left + right); eauto); reflexivity.
     Unshelve. all: auto.
 Qed.
 
 Theorem merge'_spec :
   forall (A : LinDec) (x : A) (t1 t2 : RSTree A),
-    elem x (merge' (t1, t2)) <-> elem x t1 \/ elem x t2.
+    Elem x (merge' (t1, t2)) <-> Elem x t1 \/ Elem x t2.
 Proof.
   split; intros. elem.
-    apply elem_merge'. assumption.
-    apply elem_merge'_v2. assumption.
+    apply Elem_merge'. assumption.
+    apply Elem_merge'_v2. assumption.
 Qed.
 
-Arguments elem_merge' [A x t1 t2] _.
+Arguments Elem_merge' [A x t1 t2] _.
 
-Theorem merge'_size:
+Theorem size_merge':
   forall (A : LinDec) (t1 t2 : RSTree A),
     size (merge' (t1, t2)) = size t1 + size t2.
 Proof.
   intros. remember (t1, t2) as p. revert t1 t2 Heqp.
   functional induction @merge' A p; inv 1.
-    erewrite balance_size. cbn. rewrite (IHr r (node _ v' l' r') eq_refl).
+    erewrite size_balance. cbn. rewrite (IHr r (node _ v' l' r') eq_refl).
       cbn. lia.
-    erewrite balance_size. cbn. rewrite (IHr (node _ v l r) r' eq_refl).
+    erewrite size_balance. cbn. rewrite (IHr (node _ v l r) r' eq_refl).
       cbn. lia.
     Unshelve. all: auto.
 Qed.
 
-Theorem merge'_isHeap :
+Theorem isHeap_merge' :
   forall (A : LinDec) (t1 t2 : RSTree A),
     isHeap t1 -> isHeap t2 -> isHeap (merge' (t1, t2)).
 Proof.
   intros. remember (t1, t2) as p. revert t1 t2 Heqp H H0.
-  functional induction @merge' A p; do 3 inv 1; apply balance_isHeap; elem.
-    destruct (leqb_spec v v'); inv e0. destruct (elem_merge' H); auto.
+  functional induction @merge' A p; do 3 inv 1; apply isHeap_balance; elem.
+    destruct (leqb_spec v v'); inv e0. destruct (Elem_merge' H); auto.
       eapply leq_trans with v'. auto. inv H0.
     eapply (IHr _ _ eq_refl); auto.
-    destruct (leqb_spec v v'), (elem_merge' H); inv e0.
+    destruct (leqb_spec v v'), (Elem_merge' H); inv e0.
       eapply leq_trans with v. dec. inv H0.
     eapply (IHr _ _ eq_refl); auto.
 Qed.
 
-Theorem merge'_left_biased :
+Theorem LeftBiased_merge' :
   forall (A : LinDec) (t1 t2 : RSTree A),
-    left_biased t1 -> left_biased t2 -> left_biased (merge' (t1, t2)).
+    LeftBiased t1 -> LeftBiased t2 -> LeftBiased (merge' (t1, t2)).
 Proof.
   intros. remember (t1, t2) as p. revert t1 t2 Heqp H H0.
   functional induction @merge' A p; do 3 inv 1; cbn in *;
-  apply balance_left_biased; try eapply IHr; auto.
+  apply LeftBiased_balance; try eapply IHr; auto.
 Qed.
-
-(*Definition merge {A : LinDec} (h1 h2 : LeftistHeap A)
-  : LeftistHeap A.
-Proof.
-  destruct h1 as [t1 H11 H12], h2 as [t2 H21 H22].
-  split with (tree := @merge' A (t1, t2)).
-  apply merge'_isHeap; assumption.
-  apply merge'_left_biased; assumption.
-Defined.*)
 
 Definition insert' {A : LinDec} (x : A) (t : RSTree A) : RSTree A :=
   merge' ((singleton' x), t).
-
-(* TODO *)
-(*Definition insert {A : LinDec} (x : A) (h : LeftistHeap A)
-  : LeftistHeap A.
-Proof.
-  split with (tree := merge (singleton x) h).
-    destruct (merge _ _). cbn. assumption.
-    destruct (merge _ _). cbn. assumption.
-Defined.
-
-Theorem insert_spec :
-  forall (A : LinDec) (x y : A) (h : LeftistHeap A),
-    elem x (insert y h) <-> x = y \/ elem x h.
-Proof.
-  split; destruct h; subst; cbn; intros.
-    destruct (elem_merge' H); auto. inv H0; inv H2.
-    destruct H; subst; apply elem_merge'_v2; elem.
-Qed.*)
 
 Definition deleteMin {A : LinDec} (t : RSTree A)
   : option A * RSTree A :=
@@ -319,42 +261,42 @@ end.
 Theorem deleteMin_spec :
   forall (A : LinDec) (m : A) (t t' : RSTree A),
     isHeap t -> deleteMin t = (Some m, t') ->
-      forall x : A, elem x t' -> m ≤ x.
+      forall x : A, Elem x t' -> m ≤ x.
 Proof.
   destruct t; cbn; inversion 1; inversion 1; subst; cbn.
-  intros. destruct (elem_merge' H0); auto.
+  intros. destruct (Elem_merge' H0); auto.
 Qed.
 
-Theorem deleteMin_size:
+Theorem size_deleteMin:
   forall (A : LinDec) (m : A) (t t' : RSTree A),
     deleteMin t = (Some m, t') -> size t = S (size t').
 Proof.
-  destruct t; cbn; inversion 1; subst. rewrite merge'_size. trivial.
+  destruct t; cbn; inversion 1; subst. rewrite size_merge'. trivial.
 Qed.
 
-Theorem deleteMin_elem :
+Theorem Elem_deleteMin :
   forall (A : LinDec) (m : A) (t t' : RSTree A),
-    deleteMin t = (Some m, t') -> elem m t.
+    deleteMin t = (Some m, t') -> Elem m t.
 Proof.
   destruct t; cbn; inversion 1. constructor.
 Qed.
 
-Theorem deleteMin_isHeap :
+Theorem isHeap_deleteMin :
   forall (A : LinDec) (m : A) (t t' : RSTree A),
     isHeap t -> deleteMin t = (Some m, t') ->
       isHeap t'.
 Proof.
   destruct t; cbn; inversion 1; inversion 1; subst.
-  apply merge'_isHeap; assumption.
+  apply isHeap_merge'; assumption.
 Qed.
 
-Theorem deleteMin_left_biased :
+Theorem LeftBiased_deleteMin :
   forall (A : LinDec) (m : A) (t t' : RSTree A),
-    left_biased t -> deleteMin t = (Some m, t') ->
-      left_biased t'.
+    LeftBiased t -> deleteMin t = (Some m, t') ->
+      LeftBiased t'.
 Proof.
   destruct t; cbn; do 2 inversion 1; subst.
-  apply merge'_left_biased; assumption.
+  apply LeftBiased_merge'; assumption.
 Qed.
 
 (* Leftist heapsort *)
@@ -372,7 +314,7 @@ match deleteMin t with
 end.
 Proof.
   destruct t; cbn; inversion 1; inversion 1; subst.
-  rewrite merge'_size. lia.
+  rewrite size_merge'. lia.
 Defined.
 
 Arguments toList [x] _.
