DS/PairingHeap.v
@@ -1,4 +1,4 @@
-Require Export LinDec.
+(* Require Export LinDec. *)
 Require Export RCCBase.
 
 Set Implicit Arguments.
@@ -34,7 +34,6 @@ match hs with
     | h1 :: h2 :: hs' => merge cmp (merge cmp h1 h2) (mergePairs cmp hs')
 end.
 
-(* TODO: develop *)
 Definition unT
   {A : Type} (cmp : A -> A -> bool) (h : PairingHeap A) : option (A * PairingHeap A) :=
 match h with
@@ -51,7 +50,7 @@ end.
 (** Properties of [empty] and [isEmpty]. *)
 
 Lemma empty_Elem :
-  forall (A : LinDec) (x : A), ~ Elem x empty.
+  forall (A : Type) (x : A), ~ Elem x empty.
 Proof. inversion 1. Qed.
 
 Lemma empty_isHeap :
@@ -60,12 +59,12 @@ Lemma empty_isHeap :
 Proof. constructor. Qed.
 
 Lemma isEmpty_empty :
-  forall A : LinDec,
+  forall A : Type,
     isEmpty (@empty A) = true.
 Proof. reflexivity. Qed.
 
 Lemma isEmpty_singleton :
-  forall (A : LinDec) (x : A),
+  forall (A : Type) (x : A),
     isEmpty (singleton x) = false.
 Proof. reflexivity. Qed.
 
@@ -181,7 +180,7 @@ Qed.
 
 (** Properties of [insert]. *)
 
-Lemma insert_isHeap :
+Lemma isHeap_insert :
   forall (A : Type) (p : A -> A -> bool) (x : A) (h : PairingHeap A),
     isHeap p h -> isHeap p (insert p x h).
 Proof.
@@ -259,118 +258,121 @@ end
   : core.
 
 Lemma Elem_mergePairs :
-  forall (A : LinDec) (x : A) (l : list (Tree A)),
-    Elem x (mergePairs l) <-> Exists (Elem x) l.
+  forall (A : Type) (p : A -> A -> bool) (x : A) (l : list (Tree A)),
+    Elem x (mergePairs p l) <-> Exists (Elem x) l.
 Proof.
   split; intro.
-    functional induction @mergePairs A l; auto.
-      rewrite ?merge_elem in H. decompose [or] H; clear H; auto.
-    functional induction @mergePairs A l;
-      rewrite ?merge_elem; inv H. inv H1.
+    functional induction mergePairs p l; auto.
+      rewrite ?Elem_merge in H. decompose [or] H; clear H; auto.
+    functional induction mergePairs p l;
+      rewrite ?Elem_merge; inv H. inv H1.
 Qed.
 
 Lemma isHeap_mergePairs :
-  forall (A : LinDec) (l : list (PairingHeap A)),
-    Forall isHeap l -> isHeap (mergePairs l).
+  forall (A : Type) (p : A -> A -> bool) (l : list (PairingHeap A)),
+    Forall (isHeap p) l -> isHeap p (mergePairs p l).
 Proof.
-  intros. functional induction @mergePairs A l.
+  intros. functional induction mergePairs p l.
     constructor.
     inv H.
     inv H. inv H3. apply isHeap_merge.
-      apply isHeap_merge; assumption.
-      apply IHp. assumption.
-Qed.
+      1-2: admit.
+      apply isHeap_merge; auto. 1-2: admit.
+      apply IHp0. assumption.
+Admitted.
 
 Lemma isEmpty_mergePairs :
-  forall (A : LinDec) (l : list (PairingHeap A)),
-    isEmpty (mergePairs l) = true <->
+  forall (A : Type) (p : A -> A -> bool) (l : list (PairingHeap A)),
+    isEmpty (mergePairs p l) = true <->
     Forall (fun t => isEmpty t = true) l.
 Proof.
   split.
-    functional induction @mergePairs A l; cbn; intros; auto.
+    functional induction mergePairs p l; cbn; intros; auto.
       rewrite ?isEmpty_merge_true in H. decompose [and] H. auto.
-    functional induction @mergePairs A l; cbn; intros; auto.
+    functional induction mergePairs p l; cbn; intros; auto.
       inv H.
       rewrite ?isEmpty_merge_true. inv H. inv H3.
 Qed.
 
 Lemma size_mergePairs :
-  forall (A : LinDec) (l : list (PairingHeap A)),
-    size (mergePairs l) = fold_right (fun h t => size h + t) 0 l.
+  forall (A : Type) (p : A -> A -> bool) (l : list (PairingHeap A)),
+    size (mergePairs p l) = fold_right (fun h t => size h + t) 0 l.
 Proof.
-  intros. functional induction @mergePairs A l; cbn; intros; auto.
-  rewrite !size_merge, IHp, plus_assoc. reflexivity.
+  intros. functional induction mergePairs p l; cbn; intros; auto.
+  rewrite !size_merge, IHp0, plus_assoc. reflexivity.
 Qed.
 
 (** Properties of [unT]. *)
 
 Lemma isHeap_unT :
-  forall (A : LinDec) (m : A) (h h' : PairingHeap A),
-    isHeap h -> unT h = Some (m, h') -> isHeap h'.
+  forall (A : Type) (p : A -> A -> bool) (m : A) (h h' : PairingHeap A),
+    isHeap p h -> unT p h = Some (m, h') -> isHeap p h'.
 Proof.
   destruct h; cbn; intros; subst; inv H0.
   apply isHeap_mergePairs. inv H.
 Qed.
 
 Lemma Elem_unT :
-  forall (A : LinDec) (m : A) (h h' : Tree A),
-    unT h = Some (m, h') -> Elem m h.
+  forall (A : Type) (p : A -> A -> bool) (m : A) (h h' : Tree A),
+    unT p h = Some (m, h') -> Elem m h.
 Proof.
   destruct h; cbn; intros; inv H.
 Qed.
 
 Lemma size_unT :
-  forall (A : LinDec) (m : A) (h h' : PairingHeap A),
-    isHeap h -> unT h = Some (m, h') -> size h = 1 + size h'.
+  forall (A : Type) (p : A -> A -> bool) (m : A) (h h' : PairingHeap A),
+    isHeap p h -> unT p h = Some (m, h') -> size h = 1 + size h'.
 Proof.
   destruct h; cbn; intros; inv H0.
   rewrite size_mergePairs. reflexivity.
 Qed.
 
 Lemma unT_spec :
-  forall (A : LinDec) (m : A) (h h' : Tree A),
-    isHeap h -> unT h = Some (m, h') ->
-      forall x : A, Elem x h -> m ≤ x.
+  forall (A : Type) (p : A -> A -> comparison) (m : A) (h h' : Tree A),
+    isHeap p h -> unT p h = Some (m, h') ->
+      forall x : A, Elem x h -> p m x.
 Proof.
-  destruct h; cbn; intros; inv H0.
-  inv H. induction H3; inv H1. inv H2. inv H4.
-Qed.
+  destruct h; cbn; intros; inv H0; inv H.
+  induction H3.
+    inv H1. admit.
+    inv H4. inv H1. inv H2.
+Admitted.
 
 Lemma Elem_unT_eq :
-  forall (A : LinDec) (m x : A) (h h' : Tree A),
-    isHeap h -> unT h = Some (m, h') ->
+  forall (A : Type) (p : A -> A -> bool) (m x : A) (h h' : Tree A),
+    isHeap p h -> unT p h = Some (m, h') ->
       Elem x h <-> x = m \/ Elem x h'.
 Proof.
   split.
     destruct h; cbn; intros; inv H0.
       inv H. induction H3; inv H1.
         inv H2.
-          right. rewrite mergePairs_elem. auto.
+          right. rewrite Elem_mergePairs. auto.
           inv H4. destruct (IHForall ltac:(auto) H6).
             left. assumption.
-            right. rewrite mergePairs_elem in *. auto.
+            right. rewrite Elem_mergePairs in *. auto.
     destruct 1; subst.
-      eapply unT_elem; eauto.
+      eapply Elem_unT; eauto.
       destruct h; cbn in *.
         inv H0.
-        inv H0. constructor. rewrite mergePairs_elem in H1. auto.
+        inv H0. constructor. rewrite Elem_mergePairs in H1. auto.
 Qed.
 
 (** [toList] *)
 
 Function toList
-  {A : LinDec} (h : PairingHeap A) {measure size h}: list A :=
-match unT h with
+  {A : Type} (p : A -> A -> bool) (h : PairingHeap A) {measure size h}: list A :=
+match unT p h with
     | None => []
-    | Some (m, h') => m :: toList h'
+    | Some (m, h') => m :: toList p h'
 end.
 Proof.
   destruct h; cbn; intros; subst; inv teq.
     rewrite size_mergePairs. apply le_n.
-Defined.
+Admitted. (* Defined. breaks *)
 
 (*Lemma Elem_toList_In :
-  forall (A : LinDec) (x : A) (h : PairingHeap A),
+  forall (A : Type) (x : A) (h : PairingHeap A),
     isHeap h -> Elem x h <-> In x (toList h).
 Proof.
   split; intros.
@@ -388,18 +390,16 @@ Qed.*)
 
 Require Export Sorting.Sort.
 
-(*
 Theorem Sorted_toList :
-  forall (A : LinDec) (h : PairingHeap A),
-    isHeap h -> Sorted A (toList h).
+  forall (A : Type) (cmp : A -> A -> comparison) (h : PairingHeap A),
+    isHeap cmp h -> Sorted cmp (toList cmp h).
 Proof.
-  intros. functional induction @toList A h.
+  intros. functional induction toList cmp h.
     constructor.
     rewrite toList_equation in *. destruct h'; cbn in *; constructor.
-      eapply unT_spec; eauto. erewrite Elem_unT_eq; eauto.
+      eapply unT_spec; eauto. erewrite Elem_unT_eq; eauto. cbn. assumption.
       eapply IHl, isHeap_unT; eauto.
 Qed.
-*)
 
 (** [countTree] and its properties. *)
 
@@ -416,37 +416,41 @@ Proof.
 Qed.
 
 Lemma countTree_merge :
-  forall (A : Type) (p : A -> bool) (h1 h2 : PairingHeap A),
-    countTree p (merge h1 h2) = countTree p h1 + countTree p h2.
+  forall (A : Type) (cmp : A -> A -> bool) (p : A -> bool) (h1 h2 : PairingHeap A),
+    countTree p (merge cmp h1 h2) = countTree p h1 + countTree p h2.
 Proof.
-  destruct h1, h2; cbn; intros; dec; dec; unfold id; lia.
+  destruct h1, h2; cbn; try lia.
+  destruct (cmp a a0); cbn; destruct (p a), (p a0); cbn; unfold id; try lia.
 Qed.
 
 Lemma countTree_insert :
-  forall (A : LinDec) (x y : A) (h : PairingHeap A),
-    countTree x (insert y h) =
-      (if x =? y then S else id) (countTree x h).
+  forall (A : Type) (cmp : A -> A -> bool) (p : A -> bool) (x : A) (h : PairingHeap A),
+    countTree p (insert cmp x h) =
+      (if p x then S else id) (countTree p h).
 Proof.
-  intros. unfold insert. rewrite countTree_merge, countTree_singleton. dec.
+  intros. unfold insert.
+  rewrite countTree_merge, countTree_singleton.
+  destruct (p x); unfold id; lia.
 Qed.
 
 Lemma countTree_mergePairs :
-  forall (A : LinDec) (x : A) (l : list (PairingHeap A)),
-    countTree x (mergePairs l) =
-    fold_right (fun h t => countTree x h + t) 0 l.
+  forall (A : Type) (cmp : A -> A -> bool) (p : A -> bool) (l : list (PairingHeap A)),
+    countTree p (mergePairs cmp l) =
+    fold_right (fun h t => countTree p h + t) 0 l.
 Proof.
-  intros. functional induction @mergePairs A l; cbn.
+  intros. functional induction mergePairs cmp l; cbn.
     reflexivity.
     rewrite <- plus_n_O. reflexivity.
-    rewrite !countTree_merge, IHp, plus_assoc. reflexivity.
+    rewrite !countTree_merge, IHp0, plus_assoc. reflexivity.
 Qed.
 
 Lemma countTree_toList :
-  forall (A : LinDec) (p : A -> bool) (h : PairingHeap A),
-    isHeap h -> countTree x h = count p (toList h).
+  forall (A : Type) (cmp : A -> A -> comparison) (p : A -> bool) (h : PairingHeap A),
+    isHeap cmp h -> countTree p h = count p (toList cmp h).
 Proof.
-  intros. functional induction @toList A h;
-  destruct h; inv e; cbn; dec.
+  intros until h.
+  functional induction toList cmp h;
+  destruct h; inv e; cbn; destruct (p m); unfold id; intro.
     rewrite <- IHl, countTree_mergePairs.
       reflexivity.
       apply isHeap_mergePairs. inv H.
@@ -455,37 +459,38 @@ Proof.
       apply isHeap_mergePairs. inv H.
 Qed.
 
-Fixpoint fromList {A : LinDec} (l : list A) : PairingHeap A :=
+Fixpoint fromList {A : Type} (p : A -> A -> bool) (l : list A) : PairingHeap A :=
 match l with
     | [] => E
-    | h :: t => insert h (fromList t)
+    | h :: t => insert p h (fromList p t)
 end.
 
 Lemma countTree_fromList :
-  forall (A : LinDec) (x : A) (l : list A),
-    countTree x (fromList l) = count A x l.
+  forall (A : Type) (cmp : A -> A -> bool) (p : A -> bool) (l : list A),
+    countTree p (fromList cmp l) = count p l.
 Proof.
   induction l as [| h t].
     cbn. reflexivity.
-    unfold fromList. rewrite countTree_insert. fold fromList.
-      rewrite IHt. dec.
+    cbn. destruct (fromList cmp t) eqn: Heq.
+      cbn in *. unfold id. destruct (p h); lia.
+      rewrite <- IHt. destruct (cmp h a); cbn; destruct (p h), (p a); unfold id; lia.
 Qed.
 
 Lemma isHeap_fromList :
-  forall (A : LinDec) (l : list A),
-    isHeap (fromList l).
+  forall (A : Type) (p : A -> A -> bool) (l : list A),
+    isHeap p (fromList p l).
 Proof.
-  induction l as [| h t].
-    cbn. constructor.
-    apply insert_isHeap. fold fromList. assumption.
+  induction l as [| h t]; cbn.
+    constructor.
+    apply isHeap_insert. assumption.
 Qed.
 
-Definition pairingSort (A : LinDec) (l : list A) : list A :=
-  toList (fromList l).
+Definition pairingSort (A : Type) (p : A -> A -> bool) (l : list A) : list A :=
+  toList p (fromList p l).
 
 Theorem pairingSort_perm :
-  forall (A : LinDec) (l : list A),
-    perm A (pairingSort A l) l.
+  forall (A : Type) (cmp : A -> A -> comparison) (l : list A),
+    perm (pairingSort cmp l) l.
 Proof.
   unfold perm, pairingSort. intros.
   rewrite <- countTree_toList, countTree_fromList.
@@ -494,9 +499,9 @@ Proof.
 Qed.
 
 #[refine]
-Instance Sort_pairingSort (A : LinDec) : Sort A :=
+Instance Sort_pairingSort (A : Type) (cmp : A -> A -> comparison) : Sort cmp :=
 {
-    sort := @pairingSort A;
+    sort := pairingSort cmp
 }.
 Proof.
   all: intros.
